coq/well-scoped-sums/axioms.v
@@ -1,0 +1,35 @@
+(* Version: 17.09. *)
+
+(** * Axiomatic Assumptions
+    For our development, we have to extend Coq with two well known axiomatic assumptions, namely _functional extensionality_ and _propositional extensionality_. The latter entails _proof irrelevance_.
+*)
+
+(** ** Functional Extensionality
+    We import the axiom from the Coq Standard Library and derive a utility tactic to make the assumption practically usable.
+*)
+Require Import Coq.Logic.FunctionalExtensionality.
+Require Import Program.Tactics.
+
+Tactic Notation "nointr" tactic(t) :=
+  let m := fresh "marker" in
+  pose (m := tt);
+  t; revert_until m; clear m.
+
+Ltac fext := nointr repeat (
+  match goal with
+    [ |- ?x = ?y ] =>
+    (refine (@functional_extensionality_dep _ _ _ _ _) ||
+     refine (@forall_extensionality _ _ _ _) ||
+     refine (@forall_extensionalityP _ _ _ _) ||
+     refine (@forall_extensionalityS _ _ _ _)); intro
+  end).
+
+(** ** Propositional Extensionality
+    We state the axiom of _propositional extensionality_ directly and use it to prove _proof irrelevance_.
+*)
+Axiom pext : forall P Q : Prop, (P <-> Q) -> (P = Q).
+
+Lemma pi {P : Prop} (p q : P) : p = q.
+Proof.
+  assert (P = True) by (apply pext; tauto). subst. now destruct p,q.
+Qed.
