coq/well-scoped/fintype.v
@@ -1,0 +1,241 @@
+(* Version: 17.10. *)
+
+(** * Finite Types and Mappings
+    Our development utilises well-scoped de Bruijn syntax. This means that the de Bruijn indices are taken from finite types. As a consequence, any kind of substitution or environment used in conjunction with well-scoped syntax takes the form of a mapping from some finite type _I^n_. In particular, _renamings_ are mappings _I^n -> I^m_. Here we develop the theory of how these parts interact.
+*)
+Require Export axioms.
+Set Implicit Arguments.
+Unset Strict Implicit.
+
+Definition ap {X Y} (f : X -> Y) {x y : X} (p : x = y) : f x = f y :=
+  match p with eq_refl => eq_refl end.
+
+Definition apc {X Y} {f g : X -> Y} {x y : X} (p : f = g) (q : x = y) : f x = g y :=
+  match q with eq_refl => match p with eq_refl => eq_refl end end.
+
+(** ** Forward Function Composition
+    Substitutions represented as functions are ubiquitious in this development and we often have to compose them, without talking about their pointwise behaviour.
+    That is, we are interested in the forward compostion of functions, _f o g_, for which we introduce a convenient notation, "f >> g". The direction of the arrow serves as a reminder of the _forward_ nature of this composition, that is first apply _f_, then _g_. *)
+
+(** ** Finite Types
+    We implement the finite type with _n_ elements, _I^n_, as the _n_-fold iteration of the Option Type. _I^0_ is implemented as the empty type.
+*)
+
+Fixpoint fin (n : nat) : Type :=
+  match n with
+  | 0 => False
+  | S m => option (fin m)
+  end.
+
+Definition funcomp {X Y Z} (g : Y -> Z) (f : X -> Y)  :=
+  fun x => g (f x).
+
+
+(** * Type classes for renamings. *)
+
+Class Ren1 (X1  : Type) (Y Z : Type) :=
+  ren1 : X1 -> Y -> Z.
+
+Class Ren2 (X1 X2 : Type) (Y Z : Type) :=
+  ren2 : X1 -> X2 -> Y -> Z.
+
+Class Ren3 (X1 X2 X3 : Type) (Y Z : Type) :=
+  ren3 : X1 -> X2 -> X3 -> Y -> Z.
+
+Class Ren4 (X1 X2 X3 X4 : Type) (Y Z : Type) :=
+  ren4 : X1 -> X2 -> X3 -> X4 -> Y -> Z.
+
+Class Ren5 (X1 X2 X3 X4 X5 : Type) (Y Z : Type) :=
+  ren5 : X1 -> X2 -> X3 -> X4 -> X5 -> Y -> Z.
+
+Notation "s ⟨ xi1 ⟩" := (ren1  xi1 s) (at level 7, left associativity, format "s  ⟨ xi1 ⟩") : subst_scope.
+
+Notation "s ⟨ xi1 ; xi2 ⟩" := (ren2 xi1 xi2 s) (at level 7, left associativity, format "s  ⟨ xi1 ; xi2 ⟩") : subst_scope.
+
+Notation "s ⟨ xi1 ; xi2 ; xi3 ⟩" := (ren3 xi1 xi2 xi3 s) (at level 7, left associativity, format "s  ⟨ xi1 ; xi2 ; xi3 ⟩") : subst_scope.
+
+Notation "s ⟨ xi1 ; xi2 ; xi3 ; xi4 ⟩" := (ren4  xi1 xi2 xi3 xi4 s) (at level 7, left associativity, format "s  ⟨ xi1 ; xi2 ; xi3 ; xi4 ⟩") : subst_scope.
+
+Notation "s ⟨ xi1 ; xi2 ; xi3 ; xi4 ; xi5 ⟩" := (ren5  xi1 xi2 xi3 xi4 xi5 s) (at level 7, left associativity, format "s  ⟨ xi1 ; xi2 ; xi3 ; xi4 ; xi5 ⟩") : subst_scope.
+
+Notation "⟨ xi ⟩" := (ren1 xi) (at level 1, left associativity, format "⟨ xi ⟩") : fscope.
+
+Notation "⟨ xi1 ; xi2 ⟩" := (ren2 xi1 xi2) (at level 1, left associativity, format "⟨ xi1 ; xi2 ⟩") : fscope.
+
+
+(** * Type Classes for Substiution *)
+
+Class Subst1 (X1 : Type) (Y Z: Type) :=
+  subst1 : X1 -> Y -> Z.
+
+Class Subst2 (X1 X2 : Type) (Y Z: Type) :=
+  subst2 : X1 -> X2 -> Y  -> Z.
+
+Class Subst3 (X1 X2 X3 : Type) (Y Z: Type) :=
+  subst3 : X1 -> X2 -> X3 ->  Y  -> Z.
+
+Class Subst4 (X1 X2 X3 X4: Type) (Y Z: Type) :=
+  subst4 : X1 -> X2 -> X3 -> X4 -> Y  -> Z.
+
+Class Subst5 (X1 X2 X3 X4 X5 : Type) (Y Z: Type) :=
+  subst5 : X1 -> X2 -> X3 -> X4 -> X5  -> Y  -> Z.
+
+Notation "s [ sigma ]" := (subst1 sigma s) (at level 7, left associativity, format "s '/' [ sigma ]") : subst_scope.
+
+Notation "s [ sigma ; tau ]" := (subst2 sigma tau s) (at level 7, left associativity, format "s '/' [ sigma ; '/'  tau ]") : subst_scope.
+
+
+
+Arguments funcomp {X Y Z} (g)%fscope (f)%fscope.
+
+
+Notation "f >> g" := (funcomp g f) (*fun x => g (f x)*) (at level 50).
+Open Scope subst_scope.
+
+
+(** *** Extension of Finite Mappings
+    Assume we are given a mapping _f_ from _I^n_ to some type _X_, then we can _extend_ this mapping with a new value from _x : X_ to a mapping from _I^n+1_ to _X_. We denote this operation by _x . f_ and define it as follows:
+*)
+Definition scons {X : Type} {n : nat} (x : X) (f : fin n -> X) (m : fin (S n)) : X :=
+  match m with
+  | None => x
+  | Some i => f i
+  end.
+Notation "x .: f" := (@scons _ _ x f) (at level 55) : subst_scope.
+
+(** *** Renamings and Injective Renamings
+    As mentioned above, _renamings_ are mappings between finite types.
+*)
+Definition ren (m n : nat) : Type := fin m -> fin n.
+
+
+(** We give a special name, _bound_, to the newest element in a non-empty finite type, as it usually corresponds to a freshly bound variable. We also concisely capture that _I^0_ really is empty with an exfalso proof principle. *)
+Definition var_zero {n : nat} : fin (S n) := None.
+
+Definition null {T} (i : fin 0) : T := match i with end.
+
+Definition shift {n : nat} : ren n (S n) :=
+  Some.
+
+Definition up_ren m n (xi : ren m n) : ren (S m) (S n) :=
+  var_zero .: xi >> shift.
+
+
+Definition idren {k: nat} : ren k k :=
+  fun x => x.
+
+Definition comp := @funcomp.
+
+Lemma up_ren_ren k l m (xi: ren k l) (zeta : ren l m) (rho: ren k m) (E: forall x, (xi >> zeta) x = rho x) :
+  forall x, (up_ren xi >> up_ren zeta) x = up_ren rho x.
+Proof.
+  intros [x|].
+  - simpl. unfold funcomp. now rewrite <- E.
+  - reflexivity.
+Qed.
+
+Arguments up_ren_ren {k l m} xi zeta rho E.
+
+(** Lemmas for one sort. **)
+
+(* AsimplConsEta *)
+Lemma scons_eta {T} {n : nat} (f : fin (S n) -> T) :
+  f var_zero .: shift >> f = f.
+Proof. fext. intros [x|]; reflexivity.  Qed.
+
+Definition id {X} (x : X) := x.
+
+Lemma scons_eta_id {n : nat} : var_zero .: shift = id :> (fin (S n) -> fin (S n)).
+Proof. fext. intros [x|]; reflexivity. Qed.
+
+Lemma scons_comp (T: Type) U {m} (s: T) (sigma: fin m -> T) (tau: T -> U ) :
+  (s .: sigma) >> tau = (tau s) .: (sigma >> tau) .
+Proof.
+  fext. intros [x|]. reflexivity. simpl. reflexivity.
+Qed.
+
+Ltac fsimpl :=
+  repeat match goal with
+         | [|- context[id >> ?f]] => change (id >> f) with f (* AsimplCompIdL *)
+         | [|- context[?f >> id]] => change (f >> id) with f (* AsimplCompIdR *)
+         | [|- context [id ?s]] => change (id s) with s
+         | [|- context[comp ?f ?g]] => change (comp f g) with (g >> f) (* AsimplCompIdL *)
+         | [|- context[(?f >> ?g) >> ?h]] =>
+           change ((f >> g) >> h) with (f >> (g >> h)) (* AsimplComp *)
+         | [|- context[(?s.:?sigma) var_zero]] => change ((s.:sigma) var_zero) with s
+         | [|- context[(?s.:?sigma) var_zero]] => change ((s.:sigma) var_zero) with s
+         | [|- context[(?s.:?sigma) (shift ?m)]] => change ((s.:sigma) (shift m)) with (sigma m)
+         | [|- context[idren >> ?f]] => change (idren >> f) with f
+         | [|- context[?f >> idren]] => change (f >> idren) with f
+         | [|- context[(?f >> ?g) >> ?h]] =>
+           change ((f >> g) >> h) with (f >> (g >> h))
+         | [|- context[?f >> (?x .: ?g)]] =>
+           change (f >> (x .: g)) with g
+         | [|- context[?x2 .: shift >> ?f]] =>
+           change x2 with (f var_zero); rewrite (@scons_eta _ _ f)
+         | [|- context[?f var_zero .: ?g]] =>
+           change g with (shift >> f); rewrite scons_eta
+         | _ => first [progress (rewrite scons_comp) | progress (rewrite scons_eta_id)]
+         end.
+
+Ltac fsimplc :=
+  repeat match goal with
+         | [H: context[id >> ?f] |- _] => change (id >> f) with f in H(* AsimplCompIdL *)
+         | [H: context[?f >> id]|- _] => change (f >> id) with f in H(* AsimplCompIdR *)
+         | [H: context [id ?s]|- _] => change (id s) with s in H
+         | [H: context[comp ?f ?g]|- _] => change (comp f g) with (g >> f) in H (* AsimplCompIdL *)
+         | [H: context[(?f >> ?g) >> ?h]|- _] =>
+           change ((f >> g) >> h) with (f >> (g >> h)) in H (* AsimplComp *)
+         | [H: context[(?s.:?sigma) var_zero]|- _] => change ((s.:sigma) var_zero) with s in H
+         | [H: context[(?s.:?sigma) var_zero]|- _] => change ((s.:sigma) var_zero) with s in H
+         | [H: context[(?s.:?sigma) (shift ?m)]|- _] => change ((s.:sigma) (shift m)) with (sigma m) in H
+         | [H: context[idren >> ?f]|- _] => change (idren >> f) with f in H
+         | [H: context[?f >> idren]|- _] => change (f >> idren) with f in H
+         | [H: context[(?f >> ?g) >> ?h]|- _] =>
+           change ((f >> g) >> h) with (f >> (g >> h)) in H
+         | [H: context[?f >> (?x .: ?g)]|- _] =>
+           change (f >> (x .: g)) with g in H
+         | [H: context[?x2 .: shift >> ?f]|- _] =>
+           change x2 with (f var_zero) in H; rewrite (@scons_eta _ _ f) in H
+         | [H: context[?f var_zero .: ?g]|- _] =>
+           change g with (shift >> f) in H; rewrite scons_eta in H
+         | _ => first [progress (rewrite scons_comp in *) | progress (rewrite scons_eta_id in *)]
+         end.
+
+Tactic Notation "fsimpl" "in" "*" :=
+  fsimpl; fsimplc.
+
+Opaque scons.
+Opaque var_zero.
+Opaque null.
+Opaque shift.
+Opaque up_ren.
+Opaque var_zero.
+Opaque idren.
+Opaque comp.
+Opaque funcomp.
+Opaque id.
+
+(** * Notations *)
+
+Class Var X Y :=
+  ids : X -> Y.
+
+Module CommaNotation.
+Notation "s , sigma" := (scons s sigma) (at level 60, format "s ,  sigma", right associativity) : subst_scope.
+End CommaNotation.
+
+Notation "s '..'" := (scons s ids) (at level 1, format "s ..") : subst_scope.
+
+Notation "↑" := (shift) : subst_scope.
+
+Tactic Notation "auto_case" tactic(t) :=  (match goal with
+                                           | [|- forall (i : fin 0), _] => intros []; t
+                                           | [|- forall (i : fin (S (S (S (S _))))), _] => intros [[[[|]|]|]|]; t
+                                           | [|- forall (i : fin (S (S (S _)))), _] => intros [[[|]|]|]; t
+                                           | [|- forall (i : fin (S (S _))), _] => intros [[?|]|]; t
+                                           | [|- forall (i : fin (S _)), _] =>  intros [?|]; t
+                                           end).
+    Ltac unfold_funcomp := match goal with
+                           | |-  context[(?f >> ?g) ?s] => change ((f >> g) s) with (g (f s))
+                           end.
